lean/Shars/Verification/Auxiliary.lean
@@ -29,14 +29,14 @@ theorem U64.numBits_eq_w
 := by simp +decide
 
 attribute [local simp] Std.Array.length
-attribute [-simp] List.ofFn_succ in 
+attribute [-simp] List.ofFn_succ in
 @[progress]
 theorem algos.IndexalgosStateArrayPairUsizeUsizeU64.index.spec(input: algos.StateArray)(x y: Std.Usize)
 : 5 * y.val + x.val < 25
 → ∃ output,
   index input (x,y) = .ok output ∧
   output = input.val[5 * y.val + x.val]!
-:= by 
+:= by
   intro no_overflow
   rw [index]
   progress*
@@ -49,7 +49,7 @@ theorem algos.IndexMutalgosStateArrayPairUsizeUsizeU64.index_mut.spec(input: alg
   index_mut input (x,y) = .ok (old, mk) ∧
   old = input.val[5 * y.val + x.val]! ∧
   ∀ u, (mk u).val = input.val.set (5 * y.val + x.val) u
-:= by 
+:= by
   intros
   rw [index_mut]
   /- progress* -/ -- TODO: Why does using `progress*` cause an index OOB error?
@@ -71,10 +71,10 @@ theorem BitVec.getElem!_rotateLeft(bv: BitVec n)(w: Nat)(i: Nat)
     ring
   )
 
-@[simp_lists_simps] 
+@[simp_lists_simps]
 theorem Aeneas.Std.U64.getElem!_toBits_rotate_left(u: Aeneas.Std.U64)(w: Aeneas.Std.U32)(i: Nat)
   (i_idx: i < Spec.w 6)
-: (u.rotate_left w).toBits[i]! = u.toBits[(i + Spec.w 6 - ↑w % Spec.w 6) % 64]! 
+: (u.rotate_left w).toBits[i]! = u.toBits[(i + Spec.w 6 - ↑w % Spec.w 6) % 64]!
 := by
   simp only [Spec.w, Fin.isValue, Fin.val_ofNat, Nat.reducePow, Nat.reduceMod] at *
   simp only [UScalar.toBits, List.getElem!_ofFn, i_idx, getElem!_pos, Fin.getElem_fin]
@@ -82,6 +82,461 @@ theorem Aeneas.Std.U64.getElem!_toBits_rotate_left(u: Aeneas.Std.U64)(w: Aeneas.
   simp only [Fin.getElem_fin, ←getElem!_pos]
   simp only [Aeneas.Std.UScalar.rotate_left, Std.UScalarTy.numBits]
   simp only [BitVec.getElem!_rotateLeft, i_idx]
+
+
+attribute [-simp] List.ofFn_succ
+
+@[simp]
+theorem Std.core.num.U64.toBits_to_le_bytes(u: Std.U64)
+: (Std.core.num.U64.to_le_bytes u).toBits = u.toBits
+:= by
+  simp [Std.core.num.U64.to_le_bytes, Std.Array.toBits]
+  apply List.ext_getElem
+  · simp [List.length_toBits]
+  intro i i_idx i_idx_2
+  simp at i_idx_2
+  have i_block_idx: i / 8 < 8 := by
+    apply Nat.lt_of_mul_lt_mul_left (a := 8)
+    calc _ ≤ i := by apply Nat.mul_div_le
+         i < _ := i_idx_2
+  simp [←getElem!_pos, i_block_idx, List.getElem!_toBits, List.getElem!_map]
+  simp [Std.UScalar.toBits, List.getElem!_ofFn, Nat.mod_lt, i_idx_2]
+  have :=  BitVec.toLEBytes_getElem!_testBit u.bv (i / 8) (i % 8) (by simp [Nat.mod_lt])
+  rw [Byte.testBit] at this
+  rw [BitVec.getElem_eq_testBit_toNat]
+  rw [this, Nat.div_add_mod, ←getElem!_pos]
+
+@[simp]
+theorem Std.core.num.U64.toBits_from_le_bytes(arr : Aeneas.Std.Array Std.U8 8#usize)
+: (Std.core.num.U64.from_le_bytes arr).toBits = arr.toBits
+:= by
+  rw [Std.core.num.U64.from_le_bytes, Std.Array.toBits]
+  apply List.ext_getElem
+  · simp
+  intro i i_idx i_idx2
+  simp at i_idx i_idx2
+  have i_block_idx: i / 8 < 8 := by
+    apply Nat.lt_of_mul_lt_mul_left (a := 8)
+    calc _ ≤ i := by apply Nat.mul_div_le
+         i < _ := i_idx
+  simp [←getElem!_pos, List.getElem!_toBits, Std.UScalar.toBits]
+  simp [List.getElem!_ofFn, *, Nat.mod_lt]
+  rw [Byte.testBit]
+  rw [BitVec.getElem!_eq_testBit_toNat]
+
+/- theorem Nat.add_one_div_mul_gt(a b: Nat) -/
+/- : a < (a / b + 1) * b -/
+/- := by -/
+/-   sorry -/
+
+theorem Nat.div_spec(n q: Nat){d: Nat}
+: 0 < d
+→ (q = n / d ↔ d * q ≤ n ∧ n < d * (q + 1))
+:= by
+  intro d_pos
+  apply Iff.intro
+  · rintro rfl
+    simp [Nat.mul_div_le, Nat.lt_mul_div_succ, d_pos]
+  · rintro ⟨lb, ub⟩
+    apply Nat.le_antisymm
+    · have := Nat.div_le_div_right (c := d) lb
+      rw [Nat.mul_div_cancel_left _ d_pos] at this
+      exact this
+    · have := Nat.div_lt_of_lt_mul ub
+      have := Nat.le_of_lt_add_one this
+      exact this
+
+theorem List.toBits_set(ls: List (Std.UScalar ty))(u: Std.UScalar ty)(i: Nat)
+: (ls.set i u).toBits = ls.toBits.setSlice! (i * ty.numBits) u.toBits
+:= by
+  apply List.ext_getElem
+  · simp [List.length_toBits]
+  intro j j_idx j_idx2
+  simp [←getElem!_pos]
+  simp [List.length_setSlice!, List.length_toBits] at j_idx j_idx2
+  simp [List.getElem!_toBits]
+  have numBits_pos: ty.numBits > 0 := by cases ty <;> simp
+  have j_block_idx: j / ty.numBits < ls.length := by
+    apply Nat.lt_of_mul_lt_mul_left (a := ty.numBits)
+    calc _ ≤ j := by apply Nat.mul_div_le
+         j < _ := Nat.mul_comm _ _ ▸ j_idx
+  if cond: i = j / ty.numBits then
+    subst cond
+    simp [List.getElem!_set, j_block_idx]
+    rw [List.getElem!_setSlice!_middle]
+    all_goals simp [Nat.mul_comm _ ty.numBits, ←Nat.mod_eq_sub]
+    simp [Nat.mul_div_le, Nat.mod_lt, numBits_pos, List.length_toBits, j_idx]
+  else
+    have := Nat.div_spec j i numBits_pos |>.not.mp cond
+    simp [Nat.mul_add, -not_and, not_and_or] at this
+    simp [List.getElem!_set_ne, cond, ←List.getElem!_toBits]
+    rw [List.getElem!_setSlice!_same]
+    simp
+    rw [Nat.mul_comm] at this
+    assumption
+
+theorem List.getElem!_setSlice!_eq_ite_getElem!{α : Type u_1} [Inhabited α] (s s' : List α) (i j : ℕ)
+: (s.setSlice! i s')[j]! =
+  if i ≤ j ∧ j - i < s'.length ∧ j < s.length then
+   s'[j - i]!
+  else
+   s[j]!
+:= by
+  assume j < s.length; case otherwise => simp [*, getElem!_neg]
+  if h : i ≤ j ∧ j - i < s'.length then
+    simp [h, List.getElem!_setSlice!_middle, *]
+  else
+    simp [h, *]
+    simp [-not_and, not_and_or] at h
+    rw [List.getElem!_setSlice!_same]
+    omega
+
+@[simp] theorem Aeneas.Std.UScalar.toBits_default (ty: Std.UScalarTy)
+: (default: Std.UScalar ty).toBits = (List.replicate ty.numBits false)
+:= by cases ty <;> simp +decide [default, Std.UScalar.toBits]
+
+theorem Aeneas.Std.core.num.U64.getElem_toBits_getElem_to_le_bytes(u: Std.U64)(i j: Nat)
+: j < 8
+→ (U64.to_le_bytes u).val[i]!.toBits[j]! = u.toBits[8*i + j]!
+:= by
+  -- TODO: Analyze why this kind of thing makes sense. Do we want to have this
+  -- kind of simplification? Didn't List.getELem!_toBits do quite the opposite?
+  -- TODO: Also, does this actually make use of `toBits (f bs) = toBits bs`?
+  -- I guess it also needs some kind of property over `toBits` and `getElem`.
+  -- Idk.
+  intro j_lt
+  rw [getElem!_pos]; case h => simp [UScalar.toBits, j_lt]
+  by_cases i_lt: i < 8; case neg =>
+    simp at i_lt
+    conv => lhs; arg 1; rw [getElem!_neg (h := by simp [i_lt])]
+    conv => rhs; rw [getElem!_neg (h := by
+      simp [UScalar.toBits]
+      have: 8 * i ≥ 64 := Nat.mul_le_mul_left 8 i_lt
+      omega
+    )]
+    simp only [UScalar.toBits_default, List.getElem_replicate]
+    simp
+  rw [getElem!_pos]; case pos.h => simp [i_lt]
+  have ij_idx: 8 * i + j < 64 := by
+    have: 8 * i ≤ 8 * 7 := Nat.mul_le_mul_left 8 (by omega)
+    omega
+
+  rw [getElem!_pos]; case pos.h => simp [UScalar.toBits, ij_idx]
+  simp [to_le_bytes]
+  unfold Std.UScalar.toBits
+  simp
+  trans u.bv.toLEBytes[i]!.testBit j
+  · congr; rw [←getElem!_pos]
+  · rw [BitVec.toLEBytes_getElem!_testBit, ←getElem!_pos]; assumption
+
+theorem algos.StateArray.xor_byte_at.spec (input : StateArray) (byte : Std.U8) (pos : Std.Usize)
+: 8 * pos.val < 1600
+→ ∃ output,
+  xor_byte_at (input : algos.StateArray) (byte : Std.U8) (pos : Std.Usize) = .ok output ∧
+  ∀ j < output.toBits.length,
+    output.toBits[j]! = if 8*pos ≤ j ∧ j < 8*pos + 8 then (input.toBits[j]! ^^ byte.toBits[j - 8*pos]!) else input.toBits[j]!
+:= by
+  intro valid_bound
+  simp [xor_byte_at, Std.toResult] at valid_bound ⊢
+  progress*
+  intro j j_idx
+  -- Flatten the result over lists
+  simp [*, Std.Array.set, Std.Array.toBits]
+  simp [*, List.toBits_set, Std.UScalar.getElem!_xor_toBits, Std.Array.toBits]
+  simp [List.getElem!_setSlice!_eq_ite_getElem!]
+  split
+  case isTrue in_lane =>
+    -- TODO: Maybe add some a - a % b = a / b or a / b = a - a % b simplifications here
+    have j_block_eq_pos_block: j / 64 = pos.val / 8 := by
+      have := Nat.div_spec j (pos.val / 8) (show 0 < 64 from by decide) |>.mpr
+      simp +decide [Nat.mul_add] at this
+      have := this (by omega) (by omega)
+      simp [this]
+    split
+    case isTrue in_byte =>
+      simp [Std.UScalar.getElem!_xor_toBits]
+      rw [Aeneas.Std.core.num.U64.getElem_toBits_getElem_to_le_bytes]
+      case a => omega
+      have: 8 * pos.val ≤ j := by
+        rw [←Nat.div_add_mod pos.val 8]
+        simp +arith [Nat.mul_add]
+        omega
+      have: j < 8 * pos.val + 8 := by
+        rw [←Nat.div_add_mod pos.val 8]
+        simp +arith [Nat.mul_add]
+        omega
+      simp [*]
+      simp [List.getElem!_toBits]
+      congr 2
+      · simp [j_block_eq_pos_block]
+      · have: pos.val * 8 = pos.val * 8 := by rfl
+        conv at this => lhs; rw [←Nat.div_add_mod pos.val 8]; simp +arith [Nat.mul_add]; rw [Nat.mul_comm, Nat.mul_comm 8]
+        rw [Nat.sub_sub, this, Nat.add_comm]
+        conv => lhs; rw [←Nat.div_add_mod j 64, j_block_eq_pos_block]
+        conv => lhs; lhs; rhs; rw [←Nat.div_add_mod pos.val 8]
+        simp +arith [Nat.mul_add]
+        omega
+      · conv => rhs; rw [←Nat.div_add_mod pos.val 8]
+        simp +arith [Nat.mul_add]
+        omega
+    case isFalse =>
+      simp_ifs
+      simp +arith [List.getElem!_toBits, Nat.mod_eq_sub, j_block_eq_pos_block]
+  case isFalse =>
+    simp_ifs
+
+
+@[progress]
+theorem algos.StateArray.xor_lane.inner_loop.spec(i : Std.Usize)(input : Aeneas.Std.Array Std.U8 8#usize)(src : Std.Slice Std.U8)
+: src.length ≤ input.length
+→ ∃ output,
+  inner_loop i input src = .ok output ∧
+  ∀ j < output.toBits.length,
+  output.toBits[j]! = if 8*i ≤ j ∧ j < src.toBits.length then input.toBits[j]! ^^ src.toBits[j]! else input.toBits[j]!
+:= by
+  intro input_big_enough
+  unfold inner_loop
+  simp [Std.toResult]
+  progress*
+  · intro j j_idx
+    simp [*, Std.Array.set, Std.Array.toBits]
+    simp [List.toBits_set, Nat.mul_add]
+    split
+    case isTrue already_processed =>
+      simp_ifs
+      rw [List.getElem!_setSlice!_same]
+      simp
+      omega
+    case isFalse not_prev =>
+      split
+      case isTrue curr =>
+        have: i.val = j / 8 := by
+          apply Nat.div_spec j i.val (show 0 < 8 from by decide) |>.mpr
+          simp [Nat.mul_add]
+          omega
+        simp [curr] at not_prev
+        rw [List.getElem!_setSlice!_middle]; case h => simp; omega
+        simp +arith [Std.UScalar.getElem!_xor_toBits, List.getElem!_toBits, this, Nat.mod_eq_sub]
+      case isFalse not_yet =>
+        rw [List.getElem!_setSlice!_same]
+        simp
+        omega
+  · simp_ifs
+    simp
+termination_by src.toBits.length - i.val
+decreasing_by scalar_decr_tac
+
+@[progress]
+theorem algos.StateArray.xor_lane.spec(input : Std.U64) (src : Std.Slice Std.U8)
+: src.length ≤ 8
+→ ∃ output,
+  xor_lane input src = .ok output ∧
+  ∀ j < output.toBits.length,
+    output.toBits[j]! = if j < src.toBits.length then input.toBits[j]! ^^ src.toBits[j]! else input.toBits[j]!
+:= by
+  intro src_fits_in_lane
+  unfold xor_lane inner
+  simp [Std.toResult]
+  progress*
+  simp [Std.Array.toBits] at *
+  intro j j_idx
+  simp [*]
+
+attribute [scalar_tac_simps] Nat.mul_add
+
+@[progress]
+theorem algos.StateArray.xor.inner_loop.spec (input : algos.StateArray) (other : Std.Slice Std.U8) (block_idx : Std.Usize)
+: 8*block_idx.val ≤ other.val.length
+→ other.toBits.length ≤ input.toBits.length
+-- → 8 ∣ other.length
+→ ∃ output leftover,
+  inner_loop input block_idx other = .ok (output, leftover) ∧
+  leftover = other.length / 8 ∧
+  ∀ j < output.toBits.length,
+  -- TODO: This doesn't cover all of `other`, but those which are not multiples of 8
+    output.toBits[j]! = if 64 * block_idx.val ≤ j ∧ j < (other.val.take (8*leftover)).toBits.length then input.toBits[j]! ^^ other.toBits[j]! else input.toBits[j]!
+:= by
+  intro block_idx_lt input_big_enough
+  unfold inner_loop
+
+  simp [Std.toResult, Std.core.slice.index.Slice.index, Std.core.slice.index.SliceIndexRangeUsizeSlice.index]
+  progress*
+  -- TODO: This progress section is not super smooth, we handle the `index` call a bit crudely
+  simp [*, Nat.mul_add]
+  simp_ifs
+  simp
+  progress*
+  · simp[*]
+    intro j j_idx
+    simp [*, Std.Array.set, Std.Array.toBits]
+    simp [List.length_take, List.length_toBits, Nat.mul_comm 8, Nat.min_eq_left <| Nat.div_mul_le_self other.val.length 8]
+    simp [List.toBits_set]
+    split
+    case isTrue prev =>
+      simp_ifs
+      rw [List.getElem!_setSlice!_same]
+      simp; omega
+    case isFalse not_prev =>
+      simp [-not_and, not_and_or] at not_prev
+      obtain not_prev | not_prev := not_prev; swap
+      · simp_ifs
+        have: 64 * block_idx + 64 ≤ j := by
+          calc
+            _ ≤ other.length / 8 * 8 * 8 := by
+              rename i1.val ≤ other.val.length => cond
+              simp [*] at cond
+              have := Nat.div_le_div_right (c := 8) cond
+              simp at this
+              have := Nat.mul_le_mul_right 8 this
+              simp only [←Nat.mul_comm 8 (_ + _), Nat.mul_add, Nat.mul_one] at this
+              have := Nat.mul_le_mul_right 8 this
+              simp only [←Nat.mul_comm 8 (_ + _), Nat.mul_add, Nat.mul_one] at this
+              conv at this => lhs; simp +arith only
+              simp
+              assumption
+              -- TODO: PAINFUL! Work this out better.
+            _ ≤ j := by
+              simp [not_prev]
+        rw [List.getElem!_setSlice!_suffix]
+        simp [←Nat.mul_comm 64, this]
+      by_cases 64*block_idx ≤ j ∧ j < other.length * 8
+      case pos curr =>
+        have block_idx_eq_j: block_idx = j / 64 := by
+          apply Nat.div_spec j block_idx (show 0 < 64 from by decide) |>.mpr
+          omega
+        simp_ifs
+        rw [List.getElem!_setSlice!_middle]
+        case h => simp [block_idx_eq_j]; omega
+        rw [i6_post]; case a => simp; omega
+        simp_ifs
+        simp [List.getElem!_toBits]
+        simp_lists
+        simp +arith only [←Nat.mul_add_div, block_idx_eq_j, ←Nat.mod_eq_sub, Nat.div_add_mod]
+        congr 2
+        rw [Nat.mod_mod_of_dvd]
+        decide
+      case neg unprocessed =>
+        simp_ifs
+        rw [List.getElem!_setSlice!_same]
+        simp [*, ←Nat.mul_comm 64]
+        scalar_tac
+  · rename_i block_idx_next_ge
+    simp [*] at block_idx_next_ge
+    simp [*]
+    constructor
+    · have := Nat.div_spec other.val.length block_idx.val ‹0 < 8›' |>.mpr (by scalar_tac)
+      exact this
+    · simp_ifs
+termination_by input.length - block_idx.val
+decreasing_by scalar_decr_tac
+
+@[simp] theorem List.toBits_take(ls: List (Aeneas.Std.UScalar ty))(n: Nat)
+: (ls.take n).toBits = ls.toBits.take (n* ty.numBits)
+:= by
+  apply List.ext_getElem
+  · simp [List.length_toBits]
+  simp [List.length_toBits, ←getElem!_pos]
+  intro i i_idx
+  by_cases cond: n ≤ ls.length
+  case pos =>
+    simp [cond] at i_idx
+    have := Nat.div_lt_of_lt_mul (Nat.mul_comm _ _ ▸ i_idx)
+    simp [List.getElem!_toBits]
+    simp_lists
+    simp [List.getElem!_toBits]
+  case neg =>
+    simp [not_le.mp] at cond
+    simp [cond, le_of_lt] at i_idx
+    have := Nat.div_lt_of_lt_mul (Nat.mul_comm _ _ ▸ i_idx)
+    have := Nat.mul_lt_mul_left (by cases ty <;> simp : 0 < ty.numBits) |>.mpr cond
+    simp [List.getElem!_toBits]
+    simp_lists
+    rw [List.take_of_length_le, List.getElem!_toBits]
+    simp [List.length_toBits, ←Nat.mul_comm ty.numBits, this, le_of_lt]
+
+@[simp] theorem List.toBits_drop(ls: List (Aeneas.Std.UScalar ty))(n: Nat)
+: (ls.drop n).toBits = ls.toBits.drop (n* ty.numBits)
+:= by
+  apply List.ext_getElem
+  · simp [List.length_toBits, Nat.sub_mul]
+  simp [List.length_toBits, Nat.sub_mul, ←getElem!_pos]
+  intro i i_idx
+  simp [List.getElem!_toBits, Nat.mul_comm n, Nat.mul_add_div (show 0 < ty.numBits from by cases ty <;> simp)]
+
+@[progress]
+theorem Aeneas.Std.core.slice.index.SliceIndexRangeFromUsizeSlice.index.spec{T : Type}
+  (r : Std.core.ops.range.RangeFrom Std.Usize)(input : Std.Slice T)
+: r.start ≤ input.length
+→  ∃ output,
+    index r input = .ok output ∧
+    output.val = input.val.drop r.start.val
+  := by
+    intro
+    unfold index
+    simp [*, Slice.drop]
+
+theorem algos.StateArray.xor.spec (input : algos.StateArray) (other : Std.Slice Std.U8)
+-- /** Assumes `other.len() < self.len() * 8` and `other.len() > 0`. */
+: other.toBits.length ≤ input.toBits.length
+→ other.length > 0
+→ ∃ output,
+  xor input other = .ok output ∧
+  ∀ j < output.toBits.length,
+    output.toBits[j]! = if j < other.toBits.length then input.toBits[j]! ^^ other.toBits[j]! else input.toBits[j]!
+:= by
+  intro input_big_enough length_other_pos
+  unfold xor inner
+  simp [Std.core.slice.index.Slice.index]
+
+  let* ⟨ processed, leftover, val_leftover, getElem!_toBits_processed ⟩ ← inner_loop.spec
+  replace val_leftover := val_leftover.symm -- To prevent simp [*] from unfolding `val_leftover`
+  let* ⟨ leftover_idx, val_leftover_idx ⟩ ← Std.Usize.mul_spec
+  split
+  case' isTrue =>
+    let* ⟨ old_lane, set_lane ⟩ ← Std.Array.index_mut_usize_spec
+    let* ⟨ rest_bytes, val_rest_bytes ⟩ ← Std.core.slice.index.SliceIndexRangeFromUsizeSlice.index.spec
+    let* ⟨ new_lane, getElem!_toBits_new_lane ⟩ ← xor_lane.spec
+  case' isFalse =>
+    skip
+
+  case isTrue =>
+    intros j j_lt
+    simp [*] at *
+    simp [*, Std.Array.set, Std.Array.toBits]
+    simp [*, List.toBits_set, List.getElem!_setSlice!_eq_ite_getElem!, List.length_toBits, List.toBits_take]
+
+    if j_processed?: j < 64*leftover then
+      -- Already processed by xor.inner
+      simp_ifs
+    else if j_new_lane?: j < 64*leftover + 64 then
+      -- This is the new case, we get into `new_lane`.
+      simp +decide only [val_leftover, not_lt] at j_processed? j_new_lane?
+      have := Nat.div_spec (n := j) (q := leftover) ‹0 < 64›' |>.mpr (by scalar_tac)
+      simp_ifs
+      simp only [this, ←Nat.mul_comm 64, ←Nat.mod_eq_sub]
+      simp [*, Nat.mod_lt]
+
+      have := List.getElem!_toBits processed.val j
+      simp at this -- The issue with having UScalar defined this way is that to not have to do these
+                    -- manipulations I need to define specialized theorems for each type.
+      rw [←this]
+
+      if j_changed_part?: j < other.val.length * 8 then
+        -- This is the part where bits were xored
+        simp [*, Std.Array.toBits, Std.Slice.toBits]
+        simp_ifs
+        simp +arith [Nat.div_add_mod]
+      else
+        -- This is the part where bits were left unchanged
+        simp [*, Std.Array.toBits, Std.Slice.toBits]
+        simp_ifs
+    else
+      simp +decide only [val_leftover] at j_processed? j_new_lane?
+      -- This section hasn't been processed yet.
+      simp_ifs
+  · simp
+    intros
+    simp [*, -val_leftover, ←val_leftover, ‹8 * (other.val.length / 8) = other.val.length›']
 
 -------------------------------------
 
